theories/Lowering/ToLinear.v
@@ -4,170 +4,6 @@ Require Import IL.
 Require Import InfinitePartition.
 Require Import SimI.
 
-Section ToLinear.
-
-  Parameter (fe: frame_env).
-  Parameter (p:inf_partition var).
-
-  Definition offset_local (x: Z) := fe.(fe_ofs_local) + 4 * x.
-  Definition idx_of_slot (x:var) := Zpos (Pos.div2 (x-1)%positive)%positive.
-  Definition toReg (x:var) :=
-    match Pos.div2 x with
-    | (1%positive) => R3
-    | (2%positive) => R4
-    | (3%positive) => R5
-    | (4%positive) => R6
-    | (5%positive) => R7
-    | (6%positive) => R8
-    | (7%positive) => R9
-    | (8%positive) => R10
-    | (9%positive) => R11
-    | (10%positive) => R12
-    | (11%positive) => R14
-    | (12%positive) => R15
-    | (13%positive) => R16
-    | (14%positive) => R17
-    | (15%positive) => R18
-    | (16%positive) => R19
-    | (17%positive) => R20
-    | (18%positive) => R21
-    | (19%positive) => R22
-    | (20%positive) => R23
-    | (21%positive) => R24
-    | (22%positive) => R25
-    | (23%positive) => R26
-    | (24%positive) => R27
-    | (25%positive) => R28
-    | (26%positive) => R29
-    | (27%positive) => R30
-    | _ => R31 (* *)
-    end.
-
-  Inductive simplOp : op -> Prop :=
-  | SCon v : simplOp (Con v)
-  | SVar x : simplOp (Var x)
-  | SNeg x : simplOp (UnOp UnOpNeg (Var x))
-  | SBinOp bop x y : simplOp (BinOp bop (Var x) (Var y))
-  .
-
-  Definition simplExp e := match e with
-                              | Operation e' => simplOp e'
-                              | _ => True
-                              end.
-
-  Definition sop := {e:op | simplOp e}.
-
-  Definition sexp := {e:exp | simplExp e}.
-
-  Inductive letKind :=
-  | LetLoad (src:Z) (dst:mreg)
-  | LetStore (src:mreg) (dst:Z)
-  | LetOpr (o:Op.operation) (srcs:list mreg) (dst:mreg)
-  | LetError.
-
-  Definition isReg x := Even.even_pos_fast x.
-
-  Definition getLetOp (r:mreg) (e:op) : letKind :=
-    match e with
-     | Con v => LetOpr (Op.Ointconst v) nil r
-     | UnOp o (Var y) =>
-       match o with
-       | UnOpToBool => LetError
-       | UnOpNeg => LetOpr Op.Onot (toReg y :: nil) r
-       end
-     | BinOp o (Var y1) (Var y2) =>
-       match o with
-       | BinOpAdd => LetOpr Op.Oadd
-       | BinOpSub => LetOpr Op.Osub
-       | BinOpMul => LetOpr Op.Omul
-       | BinOpDiv => LetOpr Op.Odiv
-       | BinOpEq  => (fun _ _ => LetError) (*PROBLEM! there is only Oxor & Onot: we 2 instructions here.*)
-       | BinOpLt  => LetOpr (Op.Ocmp (Op.Ccomp Clt))
-       end (toReg y1 :: toReg y2 :: nil) r
-     | Var y =>
-       if [ isReg y ]
-       then LetOpr Op.Omove (toReg y :: nil) r
-       else LetError
-     | _ => LetError
-    end
-  .
-
-  Definition getLetKind (x:var) (e:op) : letKind
-    := if [ isReg x ]
-       then let dst := toReg x in
-            match e with
-            | Var y => if [ isReg y ]
-                      then LetOpr (Op.Omove) (toReg y :: nil) dst
-                      else LetLoad (Zpos y) dst
-            | _ => getLetOp dst e
-            end
-       else match e with
-            | Var y => if [ isReg y ]
-                      then LetStore (toReg y) (Zpos x)
-                      else LetError
-            | _ => LetError
-            end
-  .
-
-  Definition dummyinstr := Lop Op.Omove (R3::nil) R3.
-
-  Definition toLinearCond (l:label) (e:op) : instruction :=
-    match e with
-    | Var y => Lcond (Op.Ccompimm Cne Int.zero) (toReg y :: nil) l
-    | BinOp BinOpLt (Var y1) (Var y2) => Lcond (Op.Ccomp Clt) (toReg y1 :: toReg y2 :: nil) l
-    | _ => dummyinstr
-    end
-  .
-
-  Fixpoint toLinear
-           (Λ:list label)
-           (l:label) (* the biggest label used so far *)
-           (s:stmt)
-    : code * label :=
-    match s with
-    | stmtLet x (Operation e) s =>
-      let (c', l') := toLinear Λ l s in
-      (
-        match getLetKind x e with
-        | LetLoad  src dst => Lgetstack Local src Tint dst
-        | LetStore src dst => Lsetstack src Local dst Tint
-        | LetOpr o srcs r => Lop o srcs r
-        | _ => dummyinstr
-        end :: c',
-        l'
-      )
-    | stmtLet x (Call e Y) s =>
-      toLinear Λ l s (* this is incorrect *)
-    | stmtIf e s t =>
-      let l' := Pos.succ l in
-      let (csq, lc) := toLinear Λ l' s in
-      let (alt, la) := toLinear Λ lc t in
-      (toLinearCond l' e
-                    :: alt (* we don't need to jump out,
-                              because alt's last intstruction is either Lreturn or Lgoto *)
-                    ++ Llabel l' :: csq,
-       la) (* missing jump & label *)
-    | stmtApp f Y =>
-      let l' := nth (counted f) Λ xH in
-      (Lgoto l' :: nil, l)
-    | stmtReturn (Var x) =>
-      (Lreturn::nil, l)
-    | stmtReturn _ => (Lreturn :: nil, l)
-    | stmtFun F t =>
-      let (l', Λ') := fold_left (fun (lΛ:label * list label) ps => let (l, Λ) := lΛ in
-                                                       let l' := Pos.succ l in
-                                                       (l', Λ ++ l' :: nil))
-                                F (l, Λ) in
-      let (ct, lt) := toLinear Λ' l' t in
-      fold_left (fun (cl : code * label) ps =>
-                   let (c, l)  := cl in
-                   let l' := Pos.succ l in
-                   let (c',l'') := toLinear Λ' l' (snd ps) in
-                   (c ++ Llabel l' :: c', l''))
-                F (ct, lt)
-    end.
-
-End ToLinear.
 
 Require Import Smallstep Globalenvs common.Events.
 
@@ -283,90 +119,352 @@ Instance LinearStateType G : StateType Linear.state :=
   @Build_StateType _ (linear_step_adapter G) linear_result (linear_reddec2 G)
                    (linear_int_det G) (linear_ext_det G).
 
-Lemma toLinear_correct r (L:I.labenv) I l (V:onv val) s bv vv rs m G
+Section ToLinear.
+
+  Parameter (fe: frame_env).
+  Parameter (p:inf_partition var).
+
+  Definition offset_local (x: Z) := fe.(fe_ofs_local) + 4 * x.
+  Definition toSlot (x:var) := Zpos (Pos.div2 (x-1)%positive)%positive.
+  Definition toReg (x:var) :=
+    match Pos.div2 x with
+    | (1%positive) => R3
+    | (2%positive) => R4
+    | (3%positive) => R5
+    | (4%positive) => R6
+    | (5%positive) => R7
+    | (6%positive) => R8
+    | (7%positive) => R9
+    | (8%positive) => R10
+    | (9%positive) => R11
+    | (10%positive) => R12
+    | (11%positive) => R14
+    | (12%positive) => R15
+    | (13%positive) => R16
+    | (14%positive) => R17
+    | (15%positive) => R18
+    | (16%positive) => R19
+    | (17%positive) => R20
+    | (18%positive) => R21
+    | (19%positive) => R22
+    | (20%positive) => R23
+    | (21%positive) => R24
+    | (22%positive) => R25
+    | (23%positive) => R26
+    | (24%positive) => R27
+    | (25%positive) => R28
+    | (26%positive) => R29
+    | (27%positive) => R30
+    | _ => R31 (* *)
+    end.
+
+  Inductive simplOp : op -> Prop :=
+  | SCon v : simplOp (Con v)
+  | SVar x : simplOp (Var x)
+  | SNeg x : simplOp (UnOp UnOpNeg (Var x))
+  | SBinOp bop x y : simplOp (BinOp bop (Var x) (Var y))
+  .
+
+  Definition simplExp e := match e with
+                              | Operation e' => simplOp e'
+                              | _ => False
+                              end.
+
+  Definition isReg x := Even.even_pos_fast x.
+
+  Inductive simplLet x : op -> Prop :=
+  | SimpleOp e (RG:isReg x) (SO:simplOp e) : simplLet x e
+  | SimpleStore y (RG: isReg y) (MM:~isReg x) : simplLet x (Var y).
+
+  Definition dummyinstr := Lop Op.Omove (R3::nil) R3.
+
+  Definition translateLetOp (x:var) (e:op)  :=
+    let r := toReg x in
+    match e with
+     | Con v => Lop (Op.Ointconst v) nil r::nil
+     | UnOp o (Var y) =>
+       match o with
+       | UnOpToBool => nil
+       | UnOpNeg => Lop Op.Onot (toReg y :: nil) r::nil
+       end
+     | BinOp o (Var y1) (Var y2) =>
+       match o with
+       | BinOpAdd => Lop Op.Oadd
+       | BinOpSub => Lop Op.Osub
+       | BinOpMul => Lop Op.Omul
+       | BinOpDiv => Lop Op.Odiv
+       | BinOpEq  => (fun _ _ => dummyinstr)
+       (*PROBLEM! there is only Oxor & Onot: we 2 instructions here.*)
+       | BinOpLt  => Lop (Op.Ocmp (Op.Ccomp Clt))
+       end (toReg y1 :: toReg y2 :: nil) r::nil
+     | Var y =>
+       match isReg x, isReg y with
+       | true, true => Lop Op.Omove (toReg y :: nil) r::nil
+       | false, true => Lsetstack (toReg y) Local (toSlot x) Tint::nil
+       | true, false => Lgetstack Local (toSlot y) Tint r::nil
+       | false, false => nil
+       end
+     | _ => nil
+    end
+  .
+(*
+  Definition translateLet (x:var) (e:op)
+    := if [ isReg x ]
+       then let dst := toReg x in
+            match e with
+            | Var y => if [ isReg y ]
+                      then Lop (Op.Omove) (toReg y :: nil) dst
+                      else Lgetstack Local (Zpos y) Tint dst
+            | _ => translateLetOp dst e
+            end
+       else match e with
+            | Var y => if [ isReg y ]
+                      then Lsetstack (toReg y) Local (Zpos x) Tint
+                      else dummyinstr
+            | _ => dummyinstr
+            end
+  .*)
+
+  Ltac single_step_linear := econstructor; econstructor; eauto.
+
+  Smpl Add single_step_linear : single_step.
+
+  Definition mrel V rs :=
+    forall x v, V x = Some v ->
+           Locmap.get
+             (if [isReg x] then R (toReg x) else S Local (toSlot x) Tint)
+             rs = Values.Vint v.
+
+  Smpl Add
+       match goal with
+       | [ EQ : @equiv ?V (@_eq ?V (@SOT_as_OT _ _ _)) _ _ _ |- _ ] =>
+         invc EQ
+       end : inv_trivial.
+
+  Lemma locmap_get_set_RR x v rs
+    : Locmap.get (R x) (Locmap.set (R x) v rs) = v.
+  Proof.
+    unfold Locmap.get, Locmap.set; cases; reflexivity.
+  Qed.
+
+  Lemma locmap_get_set_RS x v rs s y t
+    : Locmap.get (R x) (Locmap.set (S s y t) v rs) = Locmap.get (R x) rs.
+  Proof.
+    unfold Locmap.get, Locmap.set; repeat cases; eauto.
+  Qed.
+
+  Lemma locmap_get_set_SR x v rs s y t
+    : Locmap.get (S s y t) (Locmap.set (R x) v rs) = Locmap.get (S s y t) rs.
+  Proof.
+    unfold Locmap.get, Locmap.set; repeat cases; eauto.
+  Qed.
+
+  Local Hint Extern 1 =>
+  match goal with
+  | [ H : false = ?x, I : Is_true ?x |- _ ] => exfalso; rewrite <- H in I; inv I
+  end.
+
+  Lemma  translateLet_correct r G L V x e s bv vv l rs m (SM:simplLet x e)
+         (MR:mrel V rs)
+         (IH:forall V rs,  mrel V rs ->
+             upaco3 (@sim_gen IL.I.state _  Linear.state (LinearStateType G)) r Sim (L, V, s)
+                    (State nil bv vv l rs m))
+    :  @sim _ _ Linear.state (LinearStateType G) r Sim (L, V, stmtLet x (Operation e) s)
+            (State nil bv vv (translateLetOp x e ++ l) rs m).
+  Proof.
+    case_eq (op_eval V e); intros.
+    - unfold translateLetOp.
+      inv SM; simpl.
+      + inv SO; repeat cases;
+          pone_step; try reflexivity;
+            try (eapply IH; hnf; eauto); try intros ? ?; try cases;
+              intros; simpl in *; try monad_inv H; lud; clear_trivial_eqs;
+                try solve [exfalso; eauto
+                          | rewrite locmap_get_set_RR; eauto;
+                            rewrite <- MR; eauto; cases; eauto; try exfalso; eauto
+                          | rewrite locmap_get_set_SR;
+                            rewrite <- MR; eauto; cases; eauto; try exfalso; eauto].
+        * admit.
+        * admit.
+        * admit.
+        *
+          rewrite locmap_get_set_RR; eauto. simpl in *.
+          exploit MR as MRX; eauto; cases in MRX; unfold Locmap.get in MRX; eauto;
+            try rewrite MRX.
+          admit.
+          admit.
+        * admit.
+        * rewrite locmap_get_set_RR; eauto. simpl in *.
+          exploit MR as MRX; eauto; cases in MRX; unfold Locmap.get in MRX; eauto;
+            try rewrite MRX;
+          exploit (MR x0) as MRX'; eauto; cases in MRX'; unfold Locmap.get in MRX'; eauto;
+            try rewrite MRX';
+            simpl. invc H0. reflexivity.
+          admit. admit. admit.
+        * admit.
+        * rewrite locmap_get_set_RR; eauto. simpl in *.
+          admit.
+        * admit.
+        * admit.
+        * admit.
+        * admit.
+        * admit.
+        * admit.
+        * admit.
+        * rewrite locmap_get_set_RR; eauto. simpl in *.
+          admit.
+        * admit.
+      + repeat cases.
+        pone_step.
+        eapply IH. hnf; intros.
+        cases; lud; simpl in *; clear_trivial_eqs.
+        * invc e.
+          exfalso; eauto.
+        * unfold Locmap.get, Locmap.set.
+          repeat cases.
+          rewrite <- MR; eauto. cases. reflexivity.
+        * invc e.
+          unfold Locmap.get, Locmap.set.
+          repeat cases. simpl. exploit MR; eauto. cases in H2.
+          unfold Locmap.get in H2. cases; eauto.
+          exfalso; eauto.
+          exfalso; eauto.
+        * unfold Locmap.get, Locmap.set.
+          repeat cases.
+          exfalso. invc e. admit.
+          rewrite <- MR; eauto. cases. exfalso; eauto. reflexivity.
+          exfalso. eapply n0. hnf. admit.
+    - pno_step_left.
+  Admitted.
+
+  Definition toLinearCond (l:label) (e:op) : instruction :=
+    match e with
+    | Var y => Lcond (Op.Ccompimm Cne Int.zero) (toReg y :: nil) l
+    | BinOp BinOpLt (Var y1) (Var y2) => Lcond (Op.Ccomp Clt) (toReg y1 :: toReg y2 :: nil) l
+    | _ => dummyinstr
+    end.
+
+  Inductive simplCond : op -> Prop :=
+  | SimplCondVar x (RG:isReg x)
+    : simplCond (Var x)
+  | SimplCondLt x y (RG1:isReg x) (RG2:isReg y)
+    : simplCond (BinOp BinOpLt (Var x) (Var y)).
+
+  Fixpoint toLinear
+           (Λ:list label)
+           (l:label) (* the biggest label used so far *)
+           (s:stmt)
+    : code * label :=
+    match s with
+    | stmtLet x (Operation e) s =>
+      let (c', l') := toLinear Λ l s in
+      (translateLetOp x e ++ c', l')
+    | stmtLet x (Call e Y) s =>
+      toLinear Λ l s (* this is incorrect *)
+    | stmtIf e s t =>
+      let l' := Pos.succ l in
+      let (csq, lc) := toLinear Λ l' s in
+      let (alt, la) := toLinear Λ lc t in
+      (toLinearCond l' e
+                    :: alt (* we don't need to jump out,
+                              because alt's last intstruction is either Lreturn or Lgoto *)
+                    ++ Llabel l' :: csq,
+       la) (* missing jump & label *)
+    | stmtApp f Y =>
+      let l' := nth (counted f) Λ xH in
+      (Lgoto l' :: nil, l)
+    | stmtReturn (Var x) =>
+      (Lreturn::nil, l)
+    | stmtReturn _ => (Lreturn :: nil, l)
+    | stmtFun F t =>
+      let (l', Λ') := fold_left (fun (lΛ:label * list label) ps => let (l, Λ) := lΛ in
+                                                       let l' := Pos.succ l in
+                                                       (l', Λ ++ l' :: nil))
+                                F (l, Λ) in
+      let (ct, lt) := toLinear Λ' l' t in
+      fold_left (fun (cl : code * label) ps =>
+                   let (c, l)  := cl in
+                   let l' := Pos.succ l in
+                   let (c',l'') := toLinear Λ' l' (snd ps) in
+                   (c ++ Llabel l' :: c', l''))
+                F (ct, lt)
+    end.
+
+End ToLinear.
+
+Definition not_contains_label C l :=
+  forall n l', get C n (Llabel l') -> l' <> l.
+
+Lemma find_label_app C C' l
+  (ML: not_contains_label C l)
+  : find_label l (C ++ C') = find_label l C'.
+Proof.
+  general induction C; simpl in *; eauto.
+  cases.
+  - exfalso. destruct a; isabsurd.
+    exploit ML; eauto using get.
+    unfold is_label in Heq.
+    cases in Heq; subst; isabsurd.
+  - rewrite IHC; eauto. hnf; eauto using get.
+Qed.
+
+Lemma toLinear_correct r (L:I.labenv) I l (V:onv val) s bv vv rs m G C
+      (MR:mrel V rs)
+      (ML:not_contains_label C (Pos.succ l))
+      (CODE:fn_code bv = C ++ (fst (toLinear I l s)))
   : @sim _ _ Linear.state (LinearStateType G) r Sim (L, V, s)
          ((State nil bv vv (fst (toLinear I l s)) rs m):Linear.state).
 Proof.
-  revert L I l V s vv rs m r. pcofix CIH; intros.
-  destruct s; simpl.
-  - assert (SE:simplExp e) by admit.
-    hnf in SE.
-    destruct e; simpl.
-    + let_pair_case_eq. simpl_pair_eqs. subst.
-      case_eq (op_eval V e); intros.
-      * inv SE; simpl; unfold getLetKind; simpl; cases; simpl.
-        -- pfold; eapply SimSilent; [ eapply plus2O; single_step
-                                    | eapply plus2O; [ | eauto ]
-                                    | ].
-           econstructor. econstructor. reflexivity.
-           reflexivity.
-           right. eapply CIH.
-        -- pfold; eapply SimSilent; [ eapply plus2O; single_step
-                                    | eapply plus2O; [ | eauto ]
-                                    | ].
-           econstructor. econstructor. reflexivity.
-           reflexivity.
-           right. eapply CIH.
-        -- cases.
-           pfold; eapply SimSilent; [ eapply plus2O; single_step
-                                    | eapply plus2O; [ | eauto ]
-                                    | ].
-           econstructor. econstructor. reflexivity. reflexivity.
-           right. eapply CIH.
-           pfold; eapply SimSilent; [ eapply plus2O; single_step
-                                    | eapply plus2O; [ | eauto ]
-                                    | ].
-           econstructor. econstructor. reflexivity.
-           right. eapply CIH.
-        -- cases.
-           pfold; eapply SimSilent; [ eapply plus2O; single_step
-                                    | eapply plus2O; [ | eauto ]
-                                    | ].
-           econstructor. econstructor. reflexivity.
-           right. eapply CIH.
-           pfold; eapply SimSilent; [ eapply plus2O; single_step
-                                    | eapply plus2O; [ | eauto ]
-                                    | ].
-           econstructor. econstructor. reflexivity. reflexivity.
-           right. eapply CIH.
-        -- pfold; eapply SimSilent; [ eapply plus2O; single_step
-                                    | eapply plus2O; [ | eauto ]
-                                    | ].
-           econstructor. econstructor. reflexivity. reflexivity.
-           right. eapply CIH.
-        -- pfold; eapply SimSilent; [ eapply plus2O; single_step
-                                    | eapply plus2O; [ | eauto ]
-                                    | ].
-           econstructor. econstructor. reflexivity. reflexivity.
-           right. eapply CIH.
-        -- destruct bop;
-           try (pfold; eapply SimSilent; [ eapply plus2O; single_step
-                                    | eapply plus2O; [ econstructor; econstructor; reflexivity | eauto ]
-                                    | ];
-                right; eapply CIH).
-           pfold; eapply SimSilent; [ eapply plus2O; single_step
-                                    | eapply plus2O; [ | eauto ]
-                                    | ].
-           econstructor. econstructor. simpl.
-           simpl in *. monad_inv H.
-           admit. reflexivity.
-           right; eapply CIH.
-        -- pfold; eapply SimSilent; [ eapply plus2O; single_step
-                                    | eapply plus2O; [ | eauto ]
-                                    | ].
-           econstructor. econstructor. reflexivity.
-           reflexivity.
-           right. eapply CIH.
+  revert C L I l V s vv rs m r MR CODE ML. pcofix CIH; intros.
+  destruct s; simpl in *.
+  - cases.
+    + revert CODE. let_pair_case_eq. simpl_pair_eqs. subst. intros.
+      eapply translateLet_correct; eauto.
       * admit.
+      * intros.
+        right. eapply CIH. eauto.
+        simpl in *.
+        rewrite app_assoc in CODE. eauto.
+        admit.
     + admit.
-  - repeat (let_pair_case_eq; simpl_pair_eqs); subst. simpl.
+  - revert CODE.
+    repeat (let_pair_case_eq; simpl_pair_eqs); subst. simpl. intros.
     case_eq (op_eval V e); intros.
     + case_eq (val2bool v); intros.
-      admit.
-      admit.
-    + admit.
+      * assert (simplCond e) by admit.
+        inv H1. simpl.
+        pfold.
+        econstructor 1; try eapply plus2O.
+        -- single_step.
+        -- reflexivity.
+        -- econstructor. econstructor; only 2: reflexivity.
+           ++ simpl. simpl in *.
+             exploit MR; eauto. cases in H2. unfold Locmap.get in H2.
+             rewrite H2. simpl. admit.
+           ++ rewrite CODE. rewrite find_label_app; eauto.
+             simpl.
+             rewrite find_label_app. simpl. cases. reflexivity.
+             simpl. admit.
+        -- reflexivity.
+        -- right.
+           simpl in *.
+           eapply CIH; eauto.
+           instantiate (
+               1:=C++Lcond (Op.Ccompimm Cne Int.zero) (toReg x :: nil) (Pos.succ l)
+                     :: fst (toLinear I (snd (toLinear I (Pos.succ l) s1)) s2) ++
+                     Llabel (Pos.succ l)::nil). simpl.
+           rewrite CODE. rewrite <- !app_assoc. simpl.
+           rewrite <- !app_assoc. simpl. reflexivity.
+           admit.
+        -- admit.
+      * admit.
+    + pno_step_left.
   - admit.
-  - admit.
+  - (*pfold. econstructor 4; [| eapply star2_refl | | stuck2 | ]; swap 1 2.
+    eapply star2_silent; try eapply star2_refl.
+    destruct e; simpl; econstructor.
+    econstructor.*)
+    admit.
   - let_pair_case_eq; simpl_pair_eqs; subst.
     let_pair_case_eq; simpl_pair_eqs; subst.
     admit.
